refactored axiom args + arg order for execSt, runSt

src/Axioms_Io.v
@@ -2,14 +2,18 @@ Require Import Term ConcreteEvidence.
 
 (** IO Axioms *)
 
+Definition toRemote (t:AnnoTerm) (pTo:Plc) (e:EvidenceC) : EvidenceC.
+Admitted.
 Definition remote_events (t:AnnoTerm) (p:Plc) : (list Ev).
 Admitted.
-Definition toRemote (t:Term) (*(pTo:Plc)*) (e:EvidenceC) : EvidenceC.
-Admitted.
-Definition parallel_eval_thread (t:Term) (e:EvidenceC) : EvidenceC.
-Admitted.
 
-Definition parallel_att_vm_thread (t:AnnoTerm) (e:EvidenceC) : EvidenceC.
+(*
+Definition parallel_eval_thread (t:Term) (p:Plc) (e:EvidenceC) : EvidenceC.
+Admitted.
+*)
+
+
+Definition parallel_vm_thread (t:AnnoTerm) (p:Plc) (e:EvidenceC) : EvidenceC.
 Admitted.
 
 Definition parallel_vm_events (t:AnnoTerm) (p:Plc) : list Ev.
@@ -18,20 +22,24 @@ Admitted.
 Definition shuffled_events (el1:list Ev) (el2:list Ev) : list Ev.
 Admitted.
 
-Definition remote_evidence (t:AnnoTerm) (e:EvidenceC) : EvidenceC.
+
+
+Definition remote_evidence (t:AnnoTerm) (p:Plc) (e:EvidenceC) : EvidenceC.
 Admitted.
 
 Definition remote_trace (t:AnnoTerm) (p:Plc) : list Ev.
 Admitted.
 
-Axiom at_evidence : forall t e,
-    toRemote (unanno t) e = remote_evidence t e.
+
+
+Axiom at_evidence : forall t (p:Plc) (e:EvidenceC),
+    toRemote t p e = remote_evidence t p e.
 
 Axiom at_events : forall t p,
   remote_events t p = remote_trace t p.
 
-Axiom par_evidence : forall t e,
-    parallel_att_vm_thread t e = remote_evidence t e.
+Axiom par_evidence : forall t (p:Plc) (e:EvidenceC),
+    parallel_vm_thread t p e = remote_evidence t p e.
 
 Axiom par_events : forall t p,
   parallel_vm_events t p = remote_trace t p.
