src/External_Facts.v
@@ -1,27 +1,29 @@
-Require Import Term ConcreteEvidence StVM Impl_vm Axioms_Io.
+Require Import Term ConcreteEvidence StVM Impl_vm Axioms_Io GenStMonad.
 
 Require Import List.
 Import ListNotations.
 
 Axiom build_comp_external' : forall (t : AnnoTerm) (e : EvidenceC) (n : nat) (o : ev_store) (tr:list Ev),
-    build_comp t {| st_ev := e; st_trace := tr; st_pl := n; st_store := o |} =
+    runSt 
+      (build_comp t)
+      {| st_ev := e; st_trace := tr; st_pl := n; st_store := o |} =
     (Some tt,
-     {| st_ev := remote_evidence t e;
+     {| st_ev := remote_evidence t n e;
         st_trace := tr ++ (remote_trace t n);
         st_pl :=
           st_pl
-            (snd 
-               (build_comp t
-                           {| st_ev := e;
-                              st_trace := [];
-                              st_pl := n;
-                              st_store := o |}));
+            (
+              execSt (build_comp t)
+                     {| st_ev := e;
+                        st_trace := [];
+                        st_pl := n;
+                        st_store := o |});
         st_store :=
           st_store
-            (snd 
-               (build_comp t
-                           {| st_ev := e;
-                              st_trace := [];
-                              st_pl := n;
-                              st_store := o |}));
+            (
+              execSt (build_comp t)
+                     {| st_ev := e;
+                        st_trace := [];
+                        st_pl := n;
+                        st_store := o |});
      |}).
